trimming down the interface of Steel.Semantics.Instantiate

ulib/experimental/Steel.Semantics.Instantiate.fsti
@@ -3,11 +3,7 @@ module Steel.Semantics.Instantiate
 module S = Steel.Semantics.Hoare
 open Steel.Memory
 
-#set-options "--z3rlimit 20"
-
-let equals (p1 p2:hprop) : prop = equiv p1 p2 /\ True
-
-let state0 : S.st0 =
+type state0 : S.st0 =
   { S.heap = heap;
     S.mem = mem;
     S.hprop = hprop;
@@ -24,64 +20,9 @@ let state0 : S.st0 =
     S.emp = emp;
     S.star = star;
 
-    S.equals = equals
+    S.equals = equiv
   }
 
-val lemma_symmetry (u:unit) : Lemma (S.symmetry state0.S.equals)
+val state_obeys_st_laws (_:unit) : Lemma (S.st_laws state0)
 
-val lemma_transitive (u:unit) : Lemma (S.transitive state0.S.equals)
-
-val lemma_interp_extensionality (u:unit)
-  : Lemma (S.interp_extensionality state0.S.equals state0.S.interp)
-
-val lemma_interp_depends_only (u:unit) : Lemma (S.interp_depends_only state0)
-
-val lemma_associative (u:unit) : Lemma (S.associative state0.S.equals state0.S.star)
-
-val lemma_commutative (u:unit) : Lemma (S.commutative state0.S.equals state0.S.star)
-
-val lemma_is_unit (u:unit) : Lemma (S.is_unit state0.S.emp state0.S.equals state0.S.star)
-
-val lemma_equals_ext (u:unit) : Lemma (S.equals_ext state0.S.equals state0.S.star)
-
-val lemma_affine (u:unit) : Lemma (S.affine state0)
-
-val lemma_emp_valid (u:unit) : Lemma (S.emp_valid state0)
-
-val lemma_disjoint_sym (u:unit) : Lemma (S.disjoint_sym state0)
-
-val lemma_disjoint_join (u:unit) : Lemma (S.disjoint_join state0)
-
-val lemma_join_commutative (u:unit) : Lemma (lemma_disjoint_sym (); S.join_commutative state0)
-
-val lemma_join_associative (u:unit) : Lemma (lemma_disjoint_join(); S.join_associative state0)
-
-val lemma_weaken_depends_only_on (u:unit) : Lemma (S.weaken_depends_only_on state0)
-
-val lemma_m_implies_disjoint (u:unit) : Lemma (S.m_implies_disjoint state0)
-
-val lemma_mem_valid_locks_invariant (u:unit) : Lemma (S.mem_valid_locks_invariant state0)
-
-val lemma_valid_upd_heap (u:unit) : Lemma (lemma_m_implies_disjoint(); S.valid_upd_heap state0)
-
-let st_laws_lemma () : Lemma (S.st_laws state0) =
-  lemma_symmetry();
-  lemma_transitive();
-  lemma_interp_extensionality();
-  lemma_interp_depends_only ();
-  lemma_associative();
-  lemma_commutative();
-  lemma_is_unit();
-  lemma_equals_ext();
-  lemma_affine();
-  lemma_emp_valid();
-  lemma_disjoint_sym();
-  lemma_disjoint_join();
-  lemma_join_commutative();
-  lemma_join_associative();
-  lemma_weaken_depends_only_on();
-  lemma_m_implies_disjoint();
-  lemma_mem_valid_locks_invariant();
-  lemma_valid_upd_heap()
-
-let state : S.st = st_laws_lemma (); state0
+let state : S.st = state_obeys_st_laws (); state0
